.

Content/Solutions/NatInt_EucDiv.lean
@@ -5,3 +5,36 @@ Author: Yves Jäckle.
 -/
 
 import Mathlib.Tactic
+
+/-- The quotient of n by m in the Euclidean division-/
+def quotient (n m : ℕ) : ℕ :=
+  if h : 0 < m ∧ m ≤ n
+  then
+    have fact : n - m < n := Nat.div_rec_lemma h
+    (quotient (n - m) m) + 1
+  else
+    0
+
+/-- The remainder of n by m in the Euclidean division-/
+def remainder (n m : ℕ) : ℕ :=
+  if h : 0 < m ∧ m ≤ n
+  then
+    have fact : n - m < n := Nat.div_rec_lemma h
+    remainder (n - m) m
+  else
+    n
+
+-- The remainder is less then the divisor (is it ?)
+example (n k : ℕ) (k_pos : 0 < k) : remainder n k < k :=
+  by
+  apply @Nat.strong_induction_on (fun x => remainder x k < k) n
+  intro p ih
+  rw [remainder]
+  by_cases Q : k ≤ p
+  · rw [dif_pos ⟨k_pos,Q⟩]
+    dsimp
+    have le_lem : p - k < p := Nat.sub_lt_of_pos_le k_pos Q
+    exact ih (p-k) le_lem
+  · rw [dif_neg (not_and_of_not_right (0<k) Q)]
+    push_neg at Q
+    exact Q
